Plus

LTS.thy
@@ -23,7 +23,7 @@ that @{term "LTS_is_reachable \<Delta>"} is the reflexive, transitive closure of
 
 inductive LTS_is_reachable :: "(('q, 'a) LTS * ('q * 'q) set) \<Rightarrow> 'q \<Rightarrow> 'a list \<Rightarrow> 'q \<Rightarrow> bool" where
    LTS_Empty[intro!]:"LTS_is_reachable lts q [] q"|
-   LTS_Step1[intro!]:"(\<exists>q''. (q, q'') \<in> snd lts \<and> LTS_is_reachable lts q'' l q') \<Longrightarrow> LTS_is_reachable lts q l q'" |
+   LTS_Step1:"(\<exists>q''. (q, q'') \<in> snd lts \<and> LTS_is_reachable lts q'' l q') \<Longrightarrow> LTS_is_reachable lts q l q'" |
    LTS_Step2[intro!]:"(\<exists>q'' \<sigma>. a \<in> \<sigma> \<and> (q, \<sigma>, q'') \<in> fst lts \<and> LTS_is_reachable lts q'' w q') \<Longrightarrow> LTS_is_reachable lts q (a # w) q'"
 
 
@@ -35,7 +35,21 @@ lemma subLTSlemma:"LTS_is_reachable l1 q x y \<Longrightarrow> LTS_is_reachable 
   next
     case (LTS_Step1 q lts l q')
     then show ?case 
-      by (metis LTS_is_reachable.LTS_Step1 UnI1 snd_conv)
+      by (metis LTS_is_reachable.LTS_Step1 Un_iff snd_conv)
+  next
+    case (LTS_Step2 a q lts w q')
+    then show ?case 
+      by (smt (z3) LTS_is_reachable.LTS_Step2 UnI1 fst_conv)
+  qed
+
+lemma subLTSlemma1:"LTS_is_reachable l1 q x y \<Longrightarrow> LTS_is_reachable (fst l1 \<union> {(f q a, va, f q' a)|q va q'. (q,va,q') \<in> fst l1}, snd l1 \<union> l3) q x y"
+  proof (induction rule: LTS_is_reachable.induct)
+    case (LTS_Empty lts q)
+    then show ?case by auto
+  next
+    case (LTS_Step1 q lts l q')
+    then show ?case 
+      by (meson LTS_is_reachable.LTS_Step1 subLTSlemma)
   next
     case (LTS_Step2 a q lts w q')
     then show ?case 
@@ -49,11 +63,23 @@ lemma DeltLTSlemma1:"LTS_is_reachable lts q l q' \<Longrightarrow>LTS_is_reachab
   next
     case (LTS_Step1 q lts l q')
     then show ?case apply auto
-      by blast
+      thm LTS_Step1.IH
+      subgoal for q''
+      proof -
+        assume 1:"(q, q'') \<in> snd lts"
+        assume 2:"LTS_is_reachable lts q'' l q'"
+        assume 3:"LTS_is_reachable ({(f q a, va, f q' a) |q va q'. (q, va, q') \<in> fst lts}, {(f q a, f q' a) |q q'. (q, q') \<in> snd lts}) (f q'' a) l (f q' a)"
+        show "LTS_is_reachable ({(f q a, va, f q' a) |q va q'. (q, va, q') \<in> fst lts}, {(f q a, f q' a) |q q'. (q, q') \<in> snd lts}) (f q a) l (f q' a)"
+          using 1 2 3 LTS_Step1.IH apply auto
+          by (metis LTS_is_reachable.LTS_Step1 mem_Collect_eq pred_equals_eq2 snd_eqD)
+      qed
+      done
   next
     case (LTS_Step2 a q lts w q')
     then show ?case apply auto by blast
   qed
+
+
 
 
 lemma joinLTSlemma:"LTS_is_reachable l q x p \<Longrightarrow>  LTS_is_reachable l p y q''\<Longrightarrow> LTS_is_reachable l q (x@y) q''"
@@ -62,17 +88,16 @@ lemma joinLTSlemma:"LTS_is_reachable l q x p \<Longrightarrow>  LTS_is_reachable
     then show ?case apply auto done
   next
     case (LTS_Step1 q lts l q')
-    then show ?case by auto 
+    then show ?case 
+      by (meson LTS_is_reachable.LTS_Step1)
   next
     case (LTS_Step2 a q lts w q')
     then show ?case apply auto done
   qed
- 
-
-
-
 
 end
+
+
 (*
 text \<open> Given a set of states $\mathcal{Q}$ and an alphabet $\Sigma$,
 a labeled transition system is a subset of $\mathcal{Q} \times \Sigma
