reg2nfa.thy
@@ -8,6 +8,7 @@ section "definition of nondeterministic finite automaton"
 fun ConcatRegexp::"'v regexp \<Rightarrow> 'v regexp\<Rightarrow> 'v regexp" where
   "ConcatRegexp r1 r2 = Concat r2 r1"
 
+
 fun renameDelta1 :: "('v regexp * 'v set * 'v regexp) set \<Rightarrow> ('v regexp => 'v regexp)  \<Rightarrow> ('v regexp *'v set *'v regexp) set" where 
     "renameDelta1 ss f = {(f q,v, f q')| q v q' . (q, v, q')\<in> ss}"
 
@@ -17,20 +18,22 @@ fun renameDelta2 :: "('v regexp * 'v regexp) set \<Rightarrow> ('v regexp => 'v 
 primrec trans2LTS :: "'v regexp \<Rightarrow> 'v set \<Rightarrow> (('v regexp \<times> 'v set \<times> 'v regexp) set * ('v regexp * 'v regexp) set)" where 
     "trans2LTS (LChr v) alp_set= ({(LChr v,{v},\<epsilon>)},{})"|
     "trans2LTS (ESet) alp_set= ({(ESet,{},\<epsilon>)},{})"|
-    "trans2LTS (\<epsilon>) alp_set = ({},{})"|
+    "trans2LTS (\<epsilon>) alp_set = ({(\<epsilon>,{},\<epsilon>)},{})"|
     "trans2LTS (Dot) alp_set = ({(Dot ,alp_set, \<epsilon>)},{})"|
     "trans2LTS (Concat r1 r2) alp_set =(renameDelta1 (fst (trans2LTS r1 alp_set)) (ConcatRegexp r2) \<union> (fst (trans2LTS r2 alp_set)),
                                         (renameDelta2 (snd (trans2LTS r1 alp_set)) (ConcatRegexp r2) \<union> {(Concat r1 r2, Concat r1 r2),(Concat \<epsilon> r2, r2)}  \<union> snd (trans2LTS r2 alp_set)))"|
     "trans2LTS (Alter r1 r2) alp_set = (fst (trans2LTS r1 alp_set) \<union> fst (trans2LTS r2 alp_set), 
-                                        snd (trans2LTS r1 alp_set) \<union> snd (trans2LTS r2 alp_set) \<union> {(Alter r1 r2, r1),(Alter r1 r2, r2),(Alter r1 r2, Alter r1 r2)})"|
-    "trans2LTS (Star r) alp_set = (renameDelta1 (fst (trans2LTS r alp_set)) (ConcatRegexp (Star r)) \<union> fst (trans2LTS r alp_set), 
-                                   (renameDelta2 (snd (trans2LTS r alp_set)) (ConcatRegexp (Star r))) \<union> {(Star r, \<epsilon>),(Star r,Concat r (Star r))})"|
-    "trans2LTS (Plus r) alp_set = (renameDelta1 (fst (trans2LTS r alp_set)) (ConcatRegexp (Star r)) \<union> (fst  (renameDelta1 (fst (trans2LTS r alp_set)) (ConcatRegexp (Star r)), 
-                                   (renameDelta2 (snd (trans2LTS r alp_set)) (ConcatRegexp (Star r))) \<union> {(Star r, \<epsilon>),(Star r,Concat r (Star r))})),
-                                        (renameDelta2 (snd (trans2LTS r alp_set)) (ConcatRegexp (Star r)) \<union> {(Concat r (Star r), Concat r (Star r)),(Concat \<epsilon> (Star r), Star r)}  \<union> snd (renameDelta1 (fst (trans2LTS r alp_set)) (ConcatRegexp (Star r)), 
-                                   (renameDelta2 (snd (trans2LTS r alp_set)) (ConcatRegexp (Star r))) \<union> {(Star r, \<epsilon>),(Star r,Concat r (Star r))})))"|
+                                        snd (trans2LTS r1 alp_set) \<union> snd (trans2LTS r2 alp_set) \<union> {(Alter r1 r2, r1),(Alter r1 r2, r2)})"|
+    "trans2LTS (Star r) alp_set = (renameDelta1 (fst (trans2LTS r alp_set)) (ConcatRegexp (Star r)), 
+                                   (renameDelta2 (snd (trans2LTS r alp_set)) (ConcatRegexp (Star r))) \<union> {(Star r, \<epsilon>),(Star r,Concat r (Star r)),(Concat \<epsilon> (Star r), Star r)})"|
+    "trans2LTS (Plus r) alp_set = (renameDelta1 (renameDelta1 (fst (trans2LTS r alp_set)) (ConcatRegexp (Star r))) (ConcatRegexp (Star r)) \<union> (renameDelta1 (fst (trans2LTS r alp_set)) (ConcatRegexp (Star r))), 
+                                   {(Plus r, Concat (Concat r (Star r)) (Star r)),(Concat (Concat \<epsilon> (Star r)) (Star r),Concat (Star r) (Star r)),(Concat (Star r) (Star r), \<epsilon>),(Concat (Star r) (Star r), Star r),(Concat \<epsilon> (Star r), Concat (Star r) (Star r))}
+                                    \<union> renameDelta2 (renameDelta2 (snd (trans2LTS r alp_set)) (ConcatRegexp (Star r))) (ConcatRegexp (Star r)) \<union> (renameDelta2 (snd (trans2LTS r alp_set)) (ConcatRegexp (Star r))))"|
     "trans2LTS (Ques r) alp_set = (fst (trans2LTS r alp_set),
-                                   {(Ques r,\<epsilon>), (Ques r, r),(Ques r, Ques r)} \<union> snd (trans2LTS r alp_set))"
+                                   {(Ques r,\<epsilon>), (Ques r, r)} \<union> snd (trans2LTS r alp_set))"
+
+value "trans2LTS (Plus Dot) {v}"
+value "trans2LTS (Star Dot) {v}"
 
 primrec reg2q :: "'v regexp \<Rightarrow> 'v set\<Rightarrow>  ('v regexp) set" where
     "reg2q Dot a = {Dot, \<epsilon>}"|
@@ -62,6 +65,7 @@ theorem uniqueFinalState:"\<F> (reg2nfa r v) = {\<epsilon>}"
   apply(induct r)
   apply auto
   done
+
 
 theorem tranl_eq :
   fixes r v  
@@ -120,37 +124,33 @@ next
     apply auto
     subgoal for x
     proof -
-      assume a1:"sem_reg r1 v = {w. LTS_is_reachable (trans2LTS r1 v) r1 w ε}"
-      assume a2:"sem_reg r2 v = {w. LTS_is_reachable (trans2LTS r2 v) r2 w ε}"
-      assume a3:"LTS_is_reachable (trans2LTS r1 v) r1 x ε"
-      then show "∃q''. (q'' = r1 ∨ q'' = r2 ∨ q'' = Alter r1 r2 ∨ (Alter r1 r2, q'') ∈ snd (trans2LTS r1 v) ∨ (Alter r1 r2, q'') ∈ snd (trans2LTS r2 v)) ∧
-          LTS_is_reachable (fst (trans2LTS r1 v) ∪ fst (trans2LTS r2 v), insert (Alter r1 r2, r1) (insert (Alter r1 r2, r2) (insert (Alter r1 r2, Alter r1 r2) (snd (trans2LTS r1 v) ∪ snd (trans2LTS r2 v)))))
-           q'' x ε"
+      assume a1:"sem_reg r1 v = {w. LTS_is_reachable (trans2LTS r1 v) r1 w \<epsilon>}"
+      assume a2:"sem_reg r2 v = {w. LTS_is_reachable (trans2LTS r2 v) r2 w \<epsilon>}"
+      assume a3:"LTS_is_reachable (trans2LTS r1 v) r1 x \<epsilon>"
+      then show "LTS_is_reachable (fst (trans2LTS r1 v) \<union> fst (trans2LTS r2 v), insert (Alter r1 r2, r1) (insert (Alter r1 r2, r2) (snd (trans2LTS r1 v) \<union> snd (trans2LTS r2 v)))) (Alter r1 r2) x \<epsilon>"
      proof -
-        have c1:"LTS_is_reachable (fst (trans2LTS r1 v) ∪ fst (trans2LTS r2 v),  insert (Alter r1 r2, r1) (insert (Alter r1 r2, r2) (insert (Alter r1 r2, Alter r1 r2) (snd (trans2LTS r1 v) ∪ snd (trans2LTS r2 v))))) (Alter r1 r2) [] r1" 
+        have c1:"LTS_is_reachable (fst (trans2LTS r1 v) \<union> fst (trans2LTS r2 v), insert (Alter r1 r2, r1) (insert (Alter r1 r2, r2) (snd (trans2LTS r1 v) \<union> snd (trans2LTS r2 v)))) (Alter r1 r2) [] r1" 
           by (metis LTS_Empty LTS_Step1 insertI1 snd_conv)
-        from a3 have c2:"LTS_is_reachable (fst (trans2LTS r1 v) ∪ fst (trans2LTS r2 v),  insert (Alter r1 r2, r1) (insert (Alter r1 r2, r2) (insert (Alter r1 r2, Alter r1 r2) (snd (trans2LTS r1 v) ∪ snd (trans2LTS r2 v))))) r1 x ε"
+        from a3 have c2:"LTS_is_reachable (fst (trans2LTS r1 v) \<union> fst (trans2LTS r2 v), insert (Alter r1 r2, r1) (insert (Alter r1 r2, r2) (snd (trans2LTS r1 v) \<union> snd (trans2LTS r2 v)))) r1 x \<epsilon>"
           by (metis Un_insert_right subLTSlemma)
-        from c1 c2 have "LTS_is_reachable (fst (trans2LTS r1 v) ∪ fst (trans2LTS r2 v),  insert (Alter r1 r2, r1) (insert (Alter r1 r2, r2) (insert (Alter r1 r2, Alter r1 r2) (snd (trans2LTS r1 v) ∪ snd (trans2LTS r2 v))))) (Alter r1 r2) x ε"
+        from c1 c2 have "LTS_is_reachable (fst (trans2LTS r1 v) \<union> fst (trans2LTS r2 v), insert (Alter r1 r2, r1) (insert (Alter r1 r2, r2) (snd (trans2LTS r1 v) \<union> snd (trans2LTS r2 v)))) (Alter r1 r2) x \<epsilon>"
           by (metis LTS_Step1 insertI1 snd_eqD)
         then show ?thesis by auto
       qed
     qed
      subgoal for x
       proof -
-      assume a1:"sem_reg r1 v = {w. LTS_is_reachable (trans2LTS r1 v) r1 w ε} "
-      assume a2:"sem_reg r2 v = {w. LTS_is_reachable (trans2LTS r2 v) r2 w ε}"
-      assume a3:"LTS_is_reachable (trans2LTS r2 v) r2 x ε"
-      then show " ∃q''. (q'' = r1 ∨ q'' = r2 ∨ q'' = Alter r1 r2 ∨ (Alter r1 r2, q'') ∈ snd (trans2LTS r1 v) ∨ (Alter r1 r2, q'') ∈ snd (trans2LTS r2 v)) ∧
-          LTS_is_reachable (fst (trans2LTS r1 v) ∪ fst (trans2LTS r2 v), insert (Alter r1 r2, r1) (insert (Alter r1 r2, r2) (insert (Alter r1 r2, Alter r1 r2) (snd (trans2LTS r1 v) ∪ snd (trans2LTS r2 v)))))
-           q'' x ε"
+      assume a1:"sem_reg r1 v = {w. LTS_is_reachable (trans2LTS r1 v) r1 w \<epsilon>} "
+      assume a2:"sem_reg r2 v = {w. LTS_is_reachable (trans2LTS r2 v) r2 w \<epsilon>}"
+      assume a3:"LTS_is_reachable (trans2LTS r2 v) r2 x \<epsilon>"
+      then show "LTS_is_reachable (fst (trans2LTS r1 v) \<union> fst (trans2LTS r2 v), insert (Alter r1 r2, r1) (insert (Alter r1 r2, r2) (snd (trans2LTS r1 v) \<union> snd (trans2LTS r2 v)))) (Alter r1 r2) x \<epsilon>"
       proof -
-        have c1:"LTS_is_reachable (fst (trans2LTS r1 v) ∪ fst (trans2LTS r2 v), insert (Alter r1 r2, r1) (insert (Alter r1 r2, r2) (insert (Alter r1 r2, Alter r1 r2) (snd (trans2LTS r1 v) ∪ snd (trans2LTS r2 v))))) (Alter r1 r2) [] r2" 
+        have c1:"LTS_is_reachable (fst (trans2LTS r1 v) \<union> fst (trans2LTS r2 v), insert (Alter r1 r2, r1) (insert (Alter r1 r2, r2) (snd (trans2LTS r1 v) \<union> snd (trans2LTS r2 v)))) (Alter r1 r2) [] r2" 
           by (metis LTS_Empty LTS_Step1 insertI1 insertI2 snd_eqD)
-        have c2:"LTS_is_reachable (fst (trans2LTS r1 v) ∪ fst (trans2LTS r2 v), insert (Alter r1 r2, r1) (insert (Alter r1 r2, r2) (insert (Alter r1 r2, Alter r1 r2) (snd (trans2LTS r1 v) ∪ snd (trans2LTS r2 v))))) r2 x ε"
+        have c2:"LTS_is_reachable (fst (trans2LTS r1 v) \<union> fst (trans2LTS r2 v), insert (Alter r1 r2, r1) (insert (Alter r1 r2, r2) (snd (trans2LTS r1 v) \<union> snd (trans2LTS r2 v)))) r2 x \<epsilon>"
           using a3 
           by (smt (z3) Un_commute Un_insert_right subLTSlemma)
-        have "LTS_is_reachable (fst (trans2LTS r1 v) ∪ fst (trans2LTS r2 v), insert (Alter r1 r2, r1) (insert (Alter r1 r2, r2) (insert (Alter r1 r2, Alter r1 r2) (snd (trans2LTS r1 v) ∪ snd (trans2LTS r2 v))))) (Alter r1 r2) x ε"
+        have "LTS_is_reachable (fst (trans2LTS r1 v) \<union> fst (trans2LTS r2 v), insert (Alter r1 r2, r1) (insert (Alter r1 r2, r2) (snd (trans2LTS r1 v) \<union> snd (trans2LTS r2 v)))) (Alter r1 r2) x \<epsilon>"
           using c1 c2 
           by (metis LTS_Step1 insertI1 insertI2 snd_eqD)
         then show ?thesis by auto
@@ -166,115 +166,231 @@ next
     apply auto
     subgoal for q p
     proof -
-    assume a1:"sem_reg r1 v = {w. LTS_is_reachable (trans2LTS r1 v) r1 w ε}"
-    assume a2:"sem_reg r2 v = {w. LTS_is_reachable (trans2LTS r2 v) r2 w ε}"
-    assume a3:"LTS_is_reachable (trans2LTS r1 v) r1 q ε"
-    assume a4:"LTS_is_reachable (trans2LTS r2 v) r2 p ε"
-    show "∃q''. (q'' = Concat r1 r2 ∨ r1 = ε ∧ q'' = r2 ∨ (∃q'. q'' = Concat q' r2 ∧ (r1, q') ∈ snd (trans2LTS r1 v)) ∨ (Concat r1 r2, q'') ∈ snd (trans2LTS r2 v)) ∧
-          LTS_is_reachable
-           ({(Concat q r2, va, Concat q' r2) |q va q'. (q, va, q') ∈ fst (trans2LTS r1 v)} ∪ fst (trans2LTS r2 v),
-            insert (Concat r1 r2, Concat r1 r2) (insert (Concat ε r2, r2) ({(Concat q r2, Concat q' r2) |q q'. (q, q') ∈ snd (trans2LTS r1 v)} ∪ snd (trans2LTS r2 v))))
-           q'' (q @ p) ε"
+    assume a1:"sem_reg r1 v = {w. LTS_is_reachable (trans2LTS r1 v) r1 w \<epsilon>}"
+    assume a2:"sem_reg r2 v = {w. LTS_is_reachable (trans2LTS r2 v) r2 w \<epsilon>}"
+    assume a3:"LTS_is_reachable (trans2LTS r1 v) r1 q \<epsilon>"
+    assume a4:"LTS_is_reachable (trans2LTS r2 v) r2 p \<epsilon>"
+    show "LTS_is_reachable
+     ({(Concat q r2, va, Concat q' r2) |q va q'. (q, va, q') \<in> fst (trans2LTS r1 v)} \<union> fst (trans2LTS r2 v),
+      insert (Concat r1 r2, Concat r1 r2) (insert (Concat \<epsilon> r2, r2) ({(Concat q r2, Concat q' r2) |q q'. (q, q') \<in> snd (trans2LTS r1 v)} \<union> snd (trans2LTS r2 v))))
+     (Concat r1 r2) (q @ p) \<epsilon>"
     proof-
       have c1:"LTS_is_reachable
-     ({(Concat q r2, va, Concat q' r2) |q va q'. (q, va, q') ∈ fst (trans2LTS r1 v)},({(Concat q r2, Concat q' r2) |q q'. (q, q') ∈ snd (trans2LTS r1 v)})) (Concat r1 r2) q (Concat ε r2)"
+     ({(Concat q r2, va, Concat q' r2) |q va q'. (q, va, q') \<in> fst (trans2LTS r1 v)},({(Concat q r2, Concat q' r2) |q q'. (q, q') \<in> snd (trans2LTS r1 v)})) (Concat r1 r2) q (Concat \<epsilon> r2)"
         using a3   
         apply (induction rule: LTS_is_reachable.induct)  
         apply auto
-        apply blast
+        apply (metis (mono_tags, lifting) CollectI LTS_Step1 snd_conv)
         by blast
       then have c2:"LTS_is_reachable
-     ({(Concat q r2, va, Concat q' r2) |q va q'. (q, va, q') ∈ fst (trans2LTS r1 v)},
-            insert (Concat r1 r2, Concat r1 r2) (insert (Concat ε r2, r2) ({(Concat q r2, Concat q' r2) |q q'. (q, q') ∈ snd (trans2LTS r1 v)})))
-             (Concat r1 r2) q (Concat ε r2)"
-        apply (induction rule: LTS_is_reachable.cases) 
-        apply auto
-        apply (metis (no_types, lifting) Un_insert_right prod.sel(1) snd_eqD subLTSlemma sup_idem)
-        by (metis (no_types, lifting) Un_insert_right eq_snd_iff prod.sel(1) subLTSlemma sup_idem)
+     ({(Concat q r2, va, Concat q' r2) |q va q'. (q, va, q') \<in> fst (trans2LTS r1 v)},
+            insert (Concat r1 r2, Concat r1 r2) (insert (Concat \<epsilon> r2, r2) ({(Concat q r2, Concat q' r2) |q q'. (q, q') \<in> snd (trans2LTS r1 v)})))
+             (Concat r1 r2) q (Concat \<epsilon> r2)"
+        apply (induction rule: LTS_is_reachable.cases)
+          subgoal for lts qa
+            by auto
+          subgoal for qa lts l q'
+            apply auto
+            by (smt (z3) Un_commute c1 fst_conv insert_def snd_conv subLTSlemma sup_idem)
+          subgoal for a qa lts w q'
+            apply auto 
+            by (smt (z3) Un_commute Un_insert_left fst_conv snd_conv subLTSlemma sup_idem)
+        done
       then have c3:"LTS_is_reachable
-           ({(Concat q r2, va, Concat q' r2) |q va q'. (q, va, q') ∈ fst (trans2LTS r1 v)} ∪ fst (trans2LTS r2 v),
-            insert (Concat r1 r2, Concat r1 r2) (insert (Concat ε r2, r2) ({(Concat q r2, Concat q' r2) |q q'. (q, q') ∈ snd (trans2LTS r1 v)} ∪ snd (trans2LTS r2 v)))) (Concat r1 r2) q (Concat ε r2)"
-        apply auto
+           ({(Concat q r2, va, Concat q' r2) |q va q'. (q, va, q') \<in> fst (trans2LTS r1 v)} \<union> fst (trans2LTS r2 v),
+            insert (Concat r1 r2, Concat r1 r2) (insert (Concat \<epsilon> r2, r2) ({(Concat q r2, Concat q' r2) |q q'. (q, q') \<in> snd (trans2LTS r1 v)} \<union> snd (trans2LTS r2 v)))) (Concat r1 r2) q (Concat \<epsilon> r2)"
         by (metis (no_types, lifting) Un_insert_left fst_conv snd_eqD subLTSlemma)
       have c4:"LTS_is_reachable
-           ({(Concat q r2, va, Concat q' r2) |q va q'. (q, va, q') ∈ fst (trans2LTS r1 v)} ∪ fst (trans2LTS r2 v),
-            insert (Concat r1 r2, Concat r1 r2) (insert (Concat ε r2, r2) ({(Concat q r2, Concat q' r2) |q q'. (q, q') ∈ snd (trans2LTS r1 v)} ∪ snd (trans2LTS r2 v)))) (Concat ε r2) [] r2"
-        by auto
-      have c5:"LTS_is_reachable
-           ({(Concat q r2, va, Concat q' r2) |q va q'. (q, va, q') ∈ fst (trans2LTS r1 v)} ∪ fst (trans2LTS r2 v),
-            insert (Concat r1 r2, Concat r1 r2) (insert (Concat ε r2, r2) ({(Concat q r2, Concat q' r2) |q q'. (q, q') ∈ snd (trans2LTS r1 v)} ∪ snd (trans2LTS r2 v)))) r2 p ε"
+           ({(Concat q r2, va, Concat q' r2) |q va q'. (q, va, q') \<in> fst (trans2LTS r1 v)} \<union> fst (trans2LTS r2 v),
+            insert (Concat r1 r2, Concat r1 r2) (insert (Concat \<epsilon> r2, r2) ({(Concat q r2, Concat q' r2) |q q'. (q, q') \<in> snd (trans2LTS r1 v)} \<union> snd (trans2LTS r2 v)))) (Concat \<epsilon> r2) [] r2"
+        by (smt (z3) LTS_Empty LTS_Step1 insertI1 insert_commute snd_conv)
+        have c5:"LTS_is_reachable
+           ({(Concat q r2, va, Concat q' r2) |q va q'. (q, va, q') \<in> fst (trans2LTS r1 v)} \<union> fst (trans2LTS r2 v),
+            insert (Concat r1 r2, Concat r1 r2) (insert (Concat \<epsilon> r2, r2) ({(Concat q r2, Concat q' r2) |q q'. (q, q') \<in> snd (trans2LTS r1 v)} \<union> snd (trans2LTS r2 v)))) r2 p \<epsilon>"
         using a4 
         by (smt (z3) insert_def subLTSlemma sup.commute sup_left_commute)
       have "LTS_is_reachable
-           ({(Concat q r2, va, Concat q' r2) |q va q'. (q, va, q') ∈ fst (trans2LTS r1 v)} ∪ fst (trans2LTS r2 v),
-            insert (Concat r1 r2, Concat r1 r2) (insert (Concat ε r2, r2) ({(Concat q r2, Concat q' r2) |q q'. (q, q') ∈ snd (trans2LTS r1 v)} ∪ snd (trans2LTS r2 v))))
-           (Concat r1 r2) (q @ p) ε" using c3 c4 c5 
+           ({(Concat q r2, va, Concat q' r2) |q va q'. (q, va, q') \<in> fst (trans2LTS r1 v)} \<union> fst (trans2LTS r2 v),
+            insert (Concat r1 r2, Concat r1 r2) (insert (Concat \<epsilon> r2, r2) ({(Concat q r2, Concat q' r2) |q q'. (q, q') \<in> snd (trans2LTS r1 v)} \<union> snd (trans2LTS r2 v))))
+           (Concat r1 r2) (q @ p) \<epsilon>" using c3 c4 c5 
         by (smt (z3) append.right_neutral joinLTSlemma)
       thus ?thesis by auto
     qed
   qed
   subgoal for x 
   proof -
-    assume a1:"sem_reg r1 v = {w. LTS_is_reachable (trans2LTS r1 v) r1 w ε}"
-    assume a2:"sem_reg r2 v = {w. LTS_is_reachable (trans2LTS r2 v) r2 w ε}"
+    assume a1:"sem_reg r1 v = {w. LTS_is_reachable (trans2LTS r1 v) r1 w \<epsilon>}"
+    assume a2:"sem_reg r2 v = {w. LTS_is_reachable (trans2LTS r2 v) r2 w \<epsilon>}"
     assume a3:"LTS_is_reachable
-     ({(Concat q r2, va, Concat q' r2) |q va q'. (q, va, q') ∈ fst (trans2LTS r1 v)} ∪ fst (trans2LTS r2 v),
-      insert (Concat r1 r2, Concat r1 r2) (insert (Concat ε r2, r2) ({(Concat q r2, Concat q' r2) |q q'. (q, q') ∈ snd (trans2LTS r1 v)} ∪ snd (trans2LTS r2 v))))
-     (Concat r1 r2) x ε"
-    show  "∃q p. x = q @ p ∧ LTS_is_reachable (trans2LTS r1 v) r1 q ε ∧ LTS_is_reachable (trans2LTS r2 v) r2 p ε"
+     ({(Concat q r2, va, Concat q' r2) |q va q'. (q, va, q') \<in> fst (trans2LTS r1 v)} \<union> fst (trans2LTS r2 v),
+      insert (Concat r1 r2, Concat r1 r2) (insert (Concat \<epsilon> r2, r2) ({(Concat q r2, Concat q' r2) |q q'. (q, q') \<in> snd (trans2LTS r1 v)} \<union> snd (trans2LTS r2 v))))
+     (Concat r1 r2) x \<epsilon>"
+    show  "\<exists>q p. x = q @ p \<and> LTS_is_reachable (trans2LTS r1 v) r1 q \<epsilon> \<and> LTS_is_reachable (trans2LTS r2 v) r2 p \<epsilon>"
       sorry
 qed
   done
+next
+  case (Plus r)
+  then show ?case  
+    apply(unfold \<L>_def NFA_accept_def)
+    apply auto
+    subgoal for x 
+    proof -
+      assume a1:"sem_reg r v = {w. LTS_is_reachable (trans2LTS r v) r w ε}"
+      assume a2:"LTS_is_reachable (trans2LTS r v) r x ε"
+      show "LTS_is_reachable ({(Concat q (Star r), va, Concat q' (Star r)) |q va q'. ∃qa. q = Concat qa (Star r) ∧ (∃q'a. q' = Concat q'a (Star r) ∧ (qa, va, q'a) ∈ fst (trans2LTS r v))} ∪
+            {(Concat q (Star r), va, Concat q' (Star r)) |q va q'. (q, va, q') ∈ fst (trans2LTS r v)},
+            insert (Star r, ε) (insert (Star r, Concat r (Star r)) (insert (Plus r, Concat (Concat r (Star r)) (Star r)) (insert (Concat ε (Star r), Star r) {(Concat q (Star r), Concat q' (Star r)) |q q'. (q, q') ∈ snd (trans2LTS r v)}))))
+           (Plus r) x ε" 
+      proof -
+        have c1:"LTS_is_reachable ({(Concat q (Star r), va, Concat q' (Star r)) |q va q'. ∃qa. q = Concat qa (Star r) ∧ (∃q'a. q' = Concat q'a (Star r) ∧ (qa, va, q'a) ∈ fst (trans2LTS r v))} ∪
+            {(Concat q (Star r), va, Concat q' (Star r)) |q va q'. (q, va, q') ∈ fst (trans2LTS r v)},
+            insert (Star r, ε) (insert (Star r, Concat r (Star r)) (insert (Plus r, Concat (Concat r (Star r)) (Star r)) (insert (Concat ε (Star r), Star r) {(Concat q (Star r), Concat q' (Star r)) |q q'. (q, q') ∈ snd (trans2LTS r v)}))))
+              (Plus r) []  (Concat (Concat r (Star r)) (Star r))"
+          by (simp add: LTS_Empty LTS_Step1)
+
+      qed
+    subgoal for x 
+    proof -
+      assume "sem_reg r v = {w. LTS_is_reachable (trans2LTS r v) r w ε}"
+      assume "x ∈ star {w. LTS_is_reachable (trans2LTS r v) r w ε}"
+      show" LTS_is_reachable
+          ({(Concat q (Star r), va, Concat q' (Star r)) |q va q'. (q, va, q') ∈ fst (trans2LTS r v)},
+           insert (Star r, ε)
+            (insert (Star r, Concat r (Star r))
+              (insert (Concat r (Star r), Concat r (Star r)) (insert (Concat ε (Star r), Star r) {(Concat q (Star r), Concat q' (Star r)) |q q'. (q, q') ∈ snd (trans2LTS r v)}))))
+          (Plus r) x ε"
+        sorry 
+    qed
+    subgoal for x 
+    proof -
+      assume a1:" sem_reg r v = {w. LTS_is_reachable (trans2LTS r v) r w ε}"
+      assume a2:"x ∉ star {w. LTS_is_reachable (trans2LTS r v) r w ε}"
+      assume a3:"LTS_is_reachable ({(Concat q (Star r), va, Concat q' (Star r)) |q va q'. (q, va, q') ∈ fst (trans2LTS r v)},
+                  insert (Star r, ε) (insert (Star r, Concat r (Star r)) (insert (Concat r (Star r), Concat r (Star r)) (insert (Concat ε (Star r), Star r) {(Concat q (Star r), Concat q' (Star r)) |q q'. (q, q') ∈ snd (trans2LTS r v)}))))
+                 (Plus r) x ε"
+      show "LTS_is_reachable (trans2LTS r v) r x ε"
+        sorry 
+    qed
+    done
 next
   case (Star r)
   then show ?case 
      apply(unfold \<L>_def NFA_accept_def)
      apply auto 
     subgoal for x 
-      sorry
-    sorry
-next
-  case (Plus r)
-  then show ?case  
-    apply(unfold \<L>_def NFA_accept_def)
-    apply auto 
-    subgoal for x 
-    
-    sorry 
-    subgoal for x 
-    
-    sorry
-    subgoal for x 
-     sorry
+    proof -
+      assume a1:"sem_reg r v = {w. LTS_is_reachable (trans2LTS r v) r w \<epsilon>}"
+      assume a2:"x \<in> star {w. LTS_is_reachable (trans2LTS r v) r w \<epsilon>}"
+      show "LTS_is_reachable
+     ({(Concat q (Star r), va, Concat q' (Star r)) |q va q'. (q, va, q') \<in> fst (trans2LTS r v)},
+      insert (Star r, \<epsilon>) (insert (Star r, Concat r (Star r)) (insert (Concat \<epsilon> (Star r), Star r) {(Concat q (Star r), Concat q' (Star r)) |q q'. (q, q') \<in> snd (trans2LTS r v)})))
+     (Star r) x \<epsilon>" 
+        using a2 proof (induction  x)
+        case zero
+        then show ?case
+          by (metis (no_types, lifting) LTS_Empty LTS_Step1 insertI1 snd_conv)
+      next
+        case (step x y)
+        then show ?case apply auto 
+        proof -
+          assume a1:"LTS_is_reachable (trans2LTS r v) r x \<epsilon>"
+          assume a2:"y \<in> star {w. LTS_is_reachable (trans2LTS r v) r w \<epsilon>}"
+          assume a3:"LTS_is_reachable ({(Concat q (Star r), va, Concat q' (Star r)) |q va q'. (q, va, q') \<in> fst (trans2LTS r v)},
+                    insert (Star r, \<epsilon>) (insert (Star r, Concat r (Star r)) (insert (Concat \<epsilon> (Star r), Star r) {(Concat q (Star r), Concat q' (Star r)) |q q'. (q, q') \<in> snd (trans2LTS r v)})))
+                   (Star r) y \<epsilon>"
+          show "LTS_is_reachable ({(Concat q (Star r), va, Concat q' (Star r)) |q va q'. (q, va, q') \<in> fst (trans2LTS r v)},
+                    insert (Star r, \<epsilon>) (insert (Star r, Concat r (Star r)) (insert (Concat \<epsilon> (Star r), Star r) {(Concat q (Star r), Concat q' (Star r)) |q q'. (q, q') \<in> snd (trans2LTS r v)})))
+                   (Star r) (x @ y) \<epsilon>"
+          proof -
+            have c1:"LTS_is_reachable ({(Concat q (Star r), va, Concat q' (Star r)) |q va q'. (q, va, q') \<in> fst (trans2LTS r v)},
+                    insert (Star r, \<epsilon>) (insert (Star r, Concat r (Star r)) (insert (Concat \<epsilon> (Star r), Star r) {(Concat q (Star r), Concat q' (Star r)) |q q'. (q, q') \<in> snd (trans2LTS r v)})))
+                    (Star r) [] (Concat r (Star r))"
+              by (smt (z3) LTS_Empty LTS_Step1 insert_iff snd_conv)
+            have c2:"LTS_is_reachable ({(Concat q (Star r), va, Concat q' (Star r)) |q va q'. (q, va, q') \<in> fst (trans2LTS r v)} , {(Concat q (Star r), Concat q' (Star r)) |q q'. (q, q') \<in> snd (trans2LTS r v)})
+                    (Concat r (Star r)) x (Concat \<epsilon> (Star r))"
+              using a1 by(simp add:DeltLTSlemma1)
+            have c4:"LTS_is_reachable ({(Concat q (Star r), va, Concat q' (Star r)) |q va q'. (q, va, q') \<in> fst (trans2LTS r v)} \<union> fst (trans2LTS r v),
+                    {(Concat q (Star r), Concat q' (Star r)) |q q'. (q, q') \<in> snd (trans2LTS r v)})
+                    (Concat r (Star r)) x (Concat \<epsilon> (Star r))"
+              using c2 by (smt (verit, best) Collect_cong Collect_disj_eq fst_eqD snd_eqD subLTSlemma)
+            have c5:"LTS_is_reachable ({(Concat q (Star r), va, Concat q' (Star r)) |q va q'. (q, va, q') \<in> fst (trans2LTS r v)} \<union> fst (trans2LTS r v),
+                     (insert (Concat \<epsilon> (Star r), Star r) {(Concat q (Star r), Concat q' (Star r)) |q q'. (q, q') \<in> snd (trans2LTS r v)}))
+                     (Concat r (Star r)) x (Concat \<epsilon> (Star r))"
+              using c4 
+              by (smt (verit, best) Collect_cong Collect_disj_eq Un_insert_right c2 fst_eqD snd_eqD subLTSlemma)
+            have c6:"LTS_is_reachable  ({(Concat q (Star r), va, Concat q' (Star r)) |q va q'. (q, va, q') \<in> fst (trans2LTS r v)} \<union> fst (trans2LTS r v),
+                    (insert (Star r, Concat r (Star r)) (insert (Concat \<epsilon> (Star r), Star r) {(Concat q (Star r), Concat q' (Star r)) |q q'. (q, q') \<in> snd (trans2LTS r v)})))
+                    (Concat r (Star r)) x (Concat \<epsilon> (Star r))"
+              using c5 by (metis (no_types, lifting) Pair_inject Un_absorb Un_insert_right prod.collapse subLTSlemma)
+            have c7:"LTS_is_reachable
+                    ({(Concat q (Star r), va, Concat q' (Star r)) |q va q'. (q, va, q') \<in> fst (trans2LTS r v)},
+                    insert (Star r, \<epsilon>) (insert (Star r, Concat r (Star r)) (insert (Concat \<epsilon> (Star r), Star r) {(Concat q (Star r), Concat q' (Star r)) |q q'. (q, q') \<in> snd (trans2LTS r v)})))
+                    (Concat r (Star r)) x (Concat \<epsilon> (Star r))"
+              by (metis (no_types, lifting) Un_insert_right c2 fst_conv snd_conv subLTSlemma sup.idem)
+            have c8:"LTS_is_reachable
+                    ({(Concat q (Star r), va, Concat q' (Star r)) |q va q'. (q, va, q') \<in> fst (trans2LTS r v)},
+                    insert (Star r, \<epsilon>) (insert (Star r, Concat r (Star r)) (insert (Concat \<epsilon> (Star r), Star r) {(Concat q (Star r), Concat q' (Star r)) |q q'. (q, q') \<in> snd (trans2LTS r v)})))
+                    (Star r) x (Concat \<epsilon> (Star r))"
+              using c1 c7 by (smt (z3) LTS_Step1 insertI1 insert_commute snd_conv)
+            have c9:"LTS_is_reachable
+                    ({(Concat q (Star r), va, Concat q' (Star r)) |q va q'. (q, va, q') \<in> fst (trans2LTS r v)},
+                    insert (Star r, \<epsilon>) (insert (Star r, Concat r (Star r)) (insert (Concat \<epsilon> (Star r), Star r) {(Concat q (Star r), Concat q' (Star r)) |q q'. (q, q') \<in> snd (trans2LTS r v)})))
+                    (Concat \<epsilon> (Star r)) [] (Star r)"
+              by (metis (no_types, lifting) LTS_Empty LTS_Step1 insertCI snd_conv)
+            have c10:"LTS_is_reachable
+                    ({(Concat q (Star r), va, Concat q' (Star r)) |q va q'. (q, va, q') \<in> fst (trans2LTS r v)},
+                    insert (Star r, \<epsilon>) (insert (Star r, Concat r (Star r)) (insert (Concat \<epsilon> (Star r), Star r) {(Concat q (Star r), Concat q' (Star r)) |q q'. (q, q') \<in> snd (trans2LTS r v)})))
+                    (Star r) x (Star r)"
+              using c8 c9 joinLTSlemma by fastforce              
+            thus ?thesis using a3 c10 joinLTSlemma 
+              by force 
+          qed
+        qed
+      qed
+    qed
+    subgoal for x sorry
     done
 next
   case (Ques r)
   then show ?case     
     apply(unfold \<L>_def NFA_accept_def)
     apply auto 
+    subgoal 
+    proof -
+      assume "sem_reg r v = {w. LTS_is_reachable (trans2LTS r v) r w \<epsilon>}"
+      show "LTS_is_reachable (fst (trans2LTS r v), insert (Ques r, \<epsilon>) (insert (Ques r, r) (snd (trans2LTS r v)))) (Ques r) [] \<epsilon>"
+        by (metis LTS_Empty LTS_Step1 insertI1 snd_conv)
+    qed
     subgoal for x
     proof -
-      assume a1:"sem_reg r v = {w. LTS_is_reachable (trans2LTS r v) r w ε}"
-      assume a2:"LTS_is_reachable (trans2LTS r v) r x ε"
-      show "∃q''. (q'' = ε ∨ q'' = r ∨ q'' = Ques r ∨ (Ques r, q'') ∈ snd (trans2LTS r v)) ∧
-          LTS_is_reachable (fst (trans2LTS r v), insert (Ques r, ε) (insert (Ques r, r) (insert (Ques r, Ques r) (snd (trans2LTS r v))))) q'' x ε"
+      assume a1:"sem_reg r v = {w. LTS_is_reachable (trans2LTS r v) r w \<epsilon>}"
+      assume a2:"LTS_is_reachable (trans2LTS r v) r x \<epsilon>"
+      show "LTS_is_reachable (fst (trans2LTS r v), insert (Ques r, \<epsilon>) (insert (Ques r, r) (snd (trans2LTS r v)))) (Ques r) x \<epsilon>"
       proof -
-        from a2 have c1:"LTS_is_reachable (fst (trans2LTS r v), insert (Ques r, ε) (insert (Ques r, r) (insert (Ques r, Ques r) (snd (trans2LTS r v))))) r x ε"
-          apply(rule LTS_is_reachable.cases)
-          apply auto
-          apply (metis Un_insert_right boolean_algebra_cancel.sup0 fst_conv snd_conv subLTSlemma)
-          by (smt (z3) Un_commute Un_insert_left fst_conv snd_conv subLTSlemma sup_idem)
-        have "LTS_is_reachable (fst (trans2LTS r v), insert (Ques r, ε) (insert (Ques r, r) (insert (Ques r, Ques r) (snd (trans2LTS r v))))) (Ques r) x ε"
-          using c1 by auto
+        from a2 have c1:"LTS_is_reachable (fst (trans2LTS r v), insert (Ques r, \<epsilon>) (insert (Ques r, r) (snd (trans2LTS r v)))) r x \<epsilon>"
+          apply(induction rule:LTS_is_reachable.induct)
+          subgoal 
+            by auto
+          subgoal for q lts l q'
+            apply auto
+            by (smt (verit, best) LTS_Step1 Un_insert_right subLTSlemma sup_idem)
+          subgoal for a q lts w q'
+            apply auto
+            by (metis Un_insert_right boolean_algebra_cancel.sup0 subLTSlemma)
+          done
+        have "LTS_is_reachable (fst (trans2LTS r v), insert (Ques r, \<epsilon>) (insert (Ques r, r) (snd (trans2LTS r v)))) (Ques r) x \<epsilon>"
+          using c1
+          by (smt (verit, best) LTS_Step1 insertI1 insert_commute snd_conv)
         thus ?thesis by auto
       qed
     qed
     subgoal for x
     proof -
-      assume a1:"sem_reg r v = {w. LTS_is_reachable (trans2LTS r v) r w ε}"
-      assume a2:"LTS_is_reachable (fst (trans2LTS r v), insert (Ques r, ε) (insert (Ques r, r) (insert (Ques r, Ques r) (snd (trans2LTS r v))))) (Ques r) x ε"
-      assume a3:"x ≠ []" 
-      show "∃q''. (r, q'') ∈ snd (trans2LTS r v) ∧ LTS_is_reachable (trans2LTS r v) q'' x ε"
+      assume a1:"sem_reg r v = {w. LTS_is_reachable (trans2LTS r v) r w \<epsilon>}"
+      assume a2:"LTS_is_reachable (fst (trans2LTS r v), insert (Ques r, \<epsilon>) (insert (Ques r, r) (snd (trans2LTS r v)))) (Ques r) x \<epsilon>"
+      assume a3:"x \<noteq> []" 
+      show "LTS_is_reachable (trans2LTS r v) r x \<epsilon>"
         sorry
     qed
     done
